

Fourier Series:

Power series convert any function into algebraic infinite series. while Fourier series convert the algebraic function into infinite no of sine and cosine series.

Fourier Series

- In many engineering problems it is necessary to express a function in a series of sines and cosine functions
- This type of series called Fourier series was first developed by the French Mathematician Joseph Fourier in ~~1822~~ 1822.

Euler's Formula

The fourier series for the function $f(x)$ interval $\alpha < x < \alpha + 2\pi$ is given by

$$f(x) = \frac{a_0}{2} + \sum_{n=1}^{\infty} a_n \cos nx + \sum_{n=1}^{\infty} b_n \sin nx \longrightarrow (1)$$

Where

$$a_0 = \frac{1}{\pi} \int_{\alpha}^{\alpha+2\pi} f(x) dx, \quad a_n = \frac{1}{\pi} \int_{\alpha}^{\alpha+2\pi} f(x) \cos nx dx \quad \& \quad b_n = \frac{1}{\pi} \int_{\alpha}^{\alpha+2\pi} f(x) \sin nx dx$$

Theorem: (Convergence of Fourier Series)

Any function $f(x)$ can be developed as a fourier series

$$f(x) = \frac{a_0}{2} + \sum_{n=1}^{\infty} a_n \cos nx + \sum_{n=1}^{\infty} b_n \sin nx$$

When a_0 , a_n & b_n are constants provided

- (i) $f(x)$ is periodic, single valued and finite
- (ii) $f(x)$ has finite no of discontinuities in any one period.
- (iii) $f(x)$ has at most a finite number of maxima and minima.

i.e. If (i), (ii), (iii) are satisfied, then the fourier series of $f(x)$ converges to $f(x)$ at all points where $f(x)$ is continuous.

Fourier Series

Periodic function \rightarrow A function $f(x)$ which satisfies the relation $f(x+T) = f(x)$ for all real x is called a periodic function. The smallest positive number T , for which this relation holds is called the period of $f(x)$.

If T be the period of $f(x)$, then $f(x) = f(x+T) = f(x+2T) = \dots = f(x+nT)$

Also $f(x) = f(x-T) = f(x-2T) = \dots = f(x-nT)$

$\therefore f(x) = f(x \pm nT)$, where 'n' is a positive integer.

Thus, $f(x)$ repeats itself after a period of T .

eg. $\sin x$, $\cos x$, $\sec x$ and $\csc x$ are the periodic function with period 2π , while $\tan x$ and $\cot x$ are the periodic function with period π ($\frac{2\pi}{n}$).

Fourier Series : If $f(x)$ be a periodic function with period 2π in the interval $a < x < a+2\pi$, then the infinite trigonometric series given by.

$$f(x) = a_0 + \sum_{n=1}^{\infty} a_n \cos nx + \sum_{n=1}^{\infty} b_n \sin nx \rightarrow \textcircled{1}$$

where a_0 , a_n & b_n are the Fourier coefficient of $f(x)$ and are determined by the following formulae

Euler Formulae

$$a_0 = \frac{1}{2\pi} \int_a^{a+2\pi} f(x) dx \rightarrow \textcircled{2}$$

$$a_n = \frac{1}{\pi} \int_a^{a+2\pi} f(x) \cos nx dx \rightarrow \textcircled{3}$$

$$b_n = \frac{1}{\pi} \int_a^{a+2\pi} f(x) \sin nx dx \rightarrow \textcircled{4}$$

If $\alpha = 0$ then interval is $0 < x < 2\pi$
and a_0, a_n & b_n are determined by the following result

$$a_0 = \frac{1}{2\pi} \int_0^{2\pi} f(x) dx$$

$$a_n = \frac{1}{\pi} \int_0^{2\pi} f(x) \cos nx dx$$

$$\& \quad b_n = \frac{1}{\pi} \int_0^{2\pi} f(x) \sin nx dx$$

→ If $f(x)$ is an even function then

→ If $f(x)$ is an odd function then

$$\int_{-a}^a f(x) dx = 2 \int_0^a f(x) dx$$

$$\int_{-a}^a f(x) dx = 0$$

Q)) Find the fourier series for the function $f(x) = e^{-ax}$, $-\pi < x < \pi$, 'a' is a constant
and hence deduce a series for $\frac{\pi}{\sinh \pi}$

Solⁿ Let the fourier series for the function $f(x) = e^{-ax}$ in $-\pi < x < \pi$ is given by

$$f(x) = a_0 + \sum_{n=1}^{\infty} a_n \cos nx + \sum_{n=1}^{\infty} b_n \sin nx \rightarrow \textcircled{1}$$

$$e^{-ax} = a_0 + \sum_{n=1}^{\infty} a_n \cos nx + \sum_{n=1}^{\infty} b_n \sin nx \rightarrow \textcircled{2}$$

If $a = -\pi$, then the interval is $-\pi < x < \pi$
and a_0, a_n & b_n are determined by the following result

$$a_0 = \frac{1}{2\pi} \int_{-\pi}^{+\pi} f(x) dx$$

$$a_n = \frac{1}{\pi} \int_{-\pi}^{+\pi} f(x) \cdot \cos nx dx$$

$$b_n = \frac{1}{\pi} \int_{-\pi}^{+\pi} f(x) \sin nx dx$$

Where a_0, a_n, b_n are Fourier constants, are to be determined by the Euler's Formulae

$$a_0 = \frac{1}{2\pi} \int_{-\pi}^{+\pi} f(x) dx$$

$$a_0 = \frac{1}{2\pi} \int_{-\pi}^{+\pi} e^{-ax} dx$$

$$= \frac{1}{2\pi} \left[\frac{e^{-ax}}{-a} \right]_{-\pi}^{+\pi} = \frac{1}{2\pi a} [e^{a\pi} - e^{-a\pi}]$$

$$a_0 = \frac{1}{\pi a} \sinh \pi a$$

Further $a_n = \frac{1}{\pi} \int_{-\pi}^{+\pi} f(x) \cos nx dx$

$$= \frac{1}{\pi} \int_{-\pi}^{+\pi} e^{-ax} \cos nx dx$$

$$= \frac{1}{\pi} \left[\frac{e^{-ax}}{a^2+n^2} (-a \cos nx + n \sin nx) \right]_{-\pi}^{+\pi}$$

$$= \frac{1}{\pi} \left[\frac{e^{-a\pi} (-a \cos n\pi + n \sin n\pi) - e^{a\pi} (-a \cos n\pi - n \sin n\pi)}{(a^2+n^2)} \right]$$

$$= \frac{1}{\pi(a^2+n^2)} [e^{-a\pi} (-a) \cos n\pi + a e^{a\pi} \cos n\pi]$$

$$= \frac{1}{\pi(a^2+n^2)} \cos n\pi (a e^{a\pi} - a e^{-a\pi})$$

$$\sin n\pi = 0$$

$$e^{ax} - e^{-ax} = 2 \sinh ax$$

$$= \frac{2a \cos n\pi \sinh a\pi}{\pi(a^2+n^2)} = \frac{2a (-1)^n \sinh a\pi}{\pi(a^2+n^2)}$$

$$\cos n\pi = (-1)^n$$

$$b_n = \frac{1}{\pi} \int_{-\pi}^{+\pi} f(x) \sin nx dx$$

$$= \frac{1}{\pi} \int_{-\pi}^{+\pi} e^{-ax} \sin nx dx$$

$$= \frac{1}{\pi} \left[\frac{e^{-ax}}{(a^2+n^2)} (-a \sin nx - n \cos nx) \right]_{-\pi}^{+\pi}$$

$$= \frac{1}{\pi} \left[\frac{e^{-a\pi}}{(a^2+n^2)} (-a \sin n\pi - n \cos n\pi) - \frac{e^{a\pi}}{(a^2+n^2)} (-a \sin n\pi - n \cos n\pi) \right]$$

$$= \frac{1}{\pi(a^2+n^2)} [e^{-a\pi} (-n \cos n\pi) + e^{a\pi} n \cos n\pi]$$

$$= \frac{1}{\pi(a^2+n^2)} n \cos n\pi (e^{a\pi} - e^{-a\pi})$$

$$= \frac{2n \cos n\pi \sinh a\pi}{\pi(a^2+n^2)}$$

$$b_n = \frac{2n (-1)^n \sinh a\pi}{\pi(a^2+n^2)}$$

Hence from (1) the Fourier series is given by

$$f(x) = a_0 + \sum a_n \cos nx + \sum b_n \sin nx$$

$$e^{-ax} = \frac{\sinh(a\pi)}{\pi a} + \sum_{n=1}^{\infty} \frac{2a (-1)^n \sinh(a\pi)}{\pi(a^2+n^2)} \cos nx$$

$$+ \sum_{n=1}^{\infty} \frac{2n (-1)^n \sinh(a\pi)}{\pi(a^2+n^2)} \sin nx$$

$$\Rightarrow \bar{e}^{ax} = \frac{\sinh(a\pi)}{a\pi} + \frac{2a \sinh(a\pi)}{\pi} \left\{ -\frac{\cos x}{1^2+a^2} + \frac{\cos 2x}{2^2+a^2} - \frac{\cos 3x}{3^2+a^2} + \dots \right\}$$

$$+ \frac{2 \sinh(a\pi)}{\pi} \left\{ -\frac{\sin x}{1^2+a^2} + \frac{2 \sin 2x}{2^2+a^2} - \frac{3 \sin 3x}{3^2+a^2} + \dots \right\}$$

put $x=0$

$$1 = \frac{\sinh(a\pi)}{a\pi} + \frac{2a \sinh(a\pi)}{\pi} \left\{ -\frac{1}{1^2+a^2} + \frac{1}{2^2+a^2} - \frac{1}{3^2+a^2} + \dots \right\} \rightarrow \textcircled{3}$$

$\therefore x=0$ is a point of continuity of $f(x) = \bar{e}^{ax}$, $-\pi < x < \pi$. So by Dirichlet's condition the series $\textcircled{3}$ will converge on $f(x) = 0 = e^0 = 1$ at $x=0$

$$\Rightarrow \frac{\pi}{\sinh(a\pi)} = \frac{1}{a} + 2a \left\{ -\frac{1}{1^2+a^2} + \frac{1}{2^2+a^2} - \frac{1}{3^2+a^2} + \dots \right\}$$

put $a=1$

$$\frac{\pi}{\sinh \pi} = 1 + 2 \left\{ -\frac{1}{2} + \frac{1}{5} - \frac{1}{10} + \frac{1}{17} - \dots \right\}$$

$$\Rightarrow \frac{\pi}{\sinh \pi} = 1 - 2 \left\{ \frac{1}{2} - \frac{1}{5} + \frac{1}{10} - \frac{1}{17} + \dots \right\}$$

Q1) Find Fourier series for the function

$$f(x) = \begin{cases} \pi + x; & -\pi < x < 0 \\ \pi - x; & 0 < x < \pi \end{cases}$$

Solⁿ

Let the Fourier series for the function

$f(x)$ in the interval $-\pi < x < \pi$ be

$$f(x) = a_0 + \sum_{n=1}^{\infty} a_n \cos nx + \sum_{n=1}^{\infty} b_n \sin nx \rightarrow (1)$$

$$a_0 = \frac{1}{2\pi} \int_{-\pi}^{+\pi} f(x) dx$$

$$= \frac{1}{2\pi} \left[\int_{-\pi}^0 f(x) dx + \int_0^{\pi} f(x) dx \right]$$

$$= \frac{1}{2\pi} \left[\int_{-\pi}^0 (\pi + x) dx + \int_0^{\pi} (\pi - x) dx \right]$$

$$= \frac{1}{2\pi} \left[\pi x + \frac{x^2}{2} \right]_{-\pi}^0 + \frac{1}{2\pi} \left[\pi x - \frac{x^2}{2} \right]_0^{\pi}$$

$$= \frac{1}{2\pi} \left[\pi^2 - \frac{\pi^2}{2} + \pi^2 - \frac{\pi^2}{2} \right] = \pi/2$$

$$a_n = \frac{1}{\pi} \int_{-\pi}^{+\pi} f(x) \cos nx dx$$

$$= \frac{1}{\pi} \left[\int_{-\pi}^0 (\pi + x) \cos nx dx + \int_0^{\pi} (\pi - x) \cos nx dx \right]$$

Integrating by parts we have

$$= \frac{1}{\pi} \left[(\pi + x) \frac{\sin nx}{n} + \frac{\cos nx}{n^2} \right]_{-\pi}^0 + \frac{1}{\pi} \left[(\pi - x) \frac{\sin nx}{n} - \frac{\cos nx}{n^2} \right]_0^{\pi}$$

$$a_n = \frac{1}{\pi} \left[\frac{1}{n^2} - \frac{\cos n\pi}{n^2} - \frac{\cos n\pi}{n^2} + \frac{1}{n^2} \right] = \frac{2}{\pi n^2} [1 - (-1)^n]$$

$\{\cos n\pi = (-1)^n\}$

$$a_n = \begin{cases} 0, & n \text{ is even} \\ \frac{4}{\pi n^2}, & n \text{ is odd} \end{cases}$$

$$b_n = \frac{1}{\pi} \int_{-\pi}^{+\pi} f(x) \sin nx dx$$

$$= \frac{1}{\pi} \left[\int_{-\pi}^0 (\pi + x) \sin nx dx + \int_0^{\pi} (\pi - x) \sin nx dx \right]$$

$$= \frac{1}{\pi} \left[\left(\frac{\pi + x}{n} \cos nx + \frac{\sin nx}{n^2} \right)_{-\pi}^0 + \frac{1}{\pi} \left[-(\pi - x) \frac{\cos nx}{n} + \frac{\sin nx}{n^2} \right]_{\pi}^0 \right]$$

$$= \frac{1}{\pi} \left[-\frac{\pi}{n} \cos 0 + \frac{2\pi \cos n\pi}{n} \right] + \frac{1}{\pi} \left[0 + \frac{\pi}{n} \cos 0 \right]$$

$$= \frac{1}{\pi} \left[-\frac{\pi}{n} + \frac{\pi}{n} \right] = 0$$

put the values a_0 , a_n & b_n in (1) we have

$$f(x) = \frac{\pi}{2} + \frac{4}{\pi} \sum_{n=1}^{\infty} \frac{\cos nx}{n^2}$$

$$= \frac{\pi}{2} + \frac{4}{\pi} \left[\frac{\cos x}{1^2} + \frac{\cos 3x}{3^2} + \dots \right]$$

Ans